simp

Semantics/Set.lean
@@ -5,41 +5,48 @@ import Mathlib.Data.Set.Defs
   # Set theorems
 -/
 
-theorem Set.mem_comprehend {α : Type} (a : α) (P : α → Prop) :
-  a ∈ ({a | P a} : Set α) ↔ P a := Iff.rfl
+theorem Set.mem_comprehend {α : Type}
+  (a : α) (P : α → Prop):
+  a ∈ ({a | P a} : Set α) ↔ P a :=
+  Iff.rfl
 
-theorem Set.mem_diff {α : Type u} {s t : Set α} (x : α) :
-  x ∈ s \ t ↔ x ∈ s ∧ x ∉ t := Iff.rfl
+theorem Set.mem_diff {α : Type u} {s t : Set α}
+  (x : α): x ∈ s \ t ↔ x ∈ s ∧ x ∉ t :=
+  Iff.rfl
 
 /-
   ### Basic subset properties
 -/
 
-theorem Subset.refl {α : Type} (x : Set α) : x ⊆ x := fun _ => id
+theorem Subset.refl {α : Type}
+  (x : Set α): x ⊆ x :=
+  λ _ => id
 
-theorem Subset.trans {α : Type} {x y z : Set α} (h1 : x ⊆ y) (h2 : y ⊆ z) : x ⊆ z :=
-  fun _ h => h2 (h1 h)
+theorem Subset.trans {α : Type} {x y z : Set α}
+  (h1 : x ⊆ y) (h2 : y ⊆ z) : x ⊆ z :=
+  λ _ h => h2 $ h1 h
 
-theorem Subset.antisymm {α : Type} {x y : Set α} (h1 : x ⊆ y) (h2 : y ⊆ x) : x = y :=
-  funext fun _ => propext ⟨fun h => h1 h, fun h => h2 h⟩
+theorem Subset.antisymm {α : Type} {x y : Set α}
+  (h1 : x ⊆ y) (h2 : y ⊆ x) : x = y :=
+  funext λ _ => propext ⟨(h1 ·), (h2 ·)⟩
 
-theorem Subset.from_eq {α : Type} {x y : Set α} (h : x = y) : x ⊆ y :=
-  fun _ h1 => h ▸ h1
+theorem Subset.from_eq {α : Type} {x y : Set α}
+  (h : x = y) : x ⊆ y :=
+  λ _ h1 => h ▸ h1
 
 /-
   ### Set if then else
 -/
 
-protected def Set.ite (t s s' : Set α) : Set α :=
+def Set.ite (t s s' : Set α): Set α :=
   s ∩ t ∪ s' \ t
 
-
-theorem Set.ite_mono (t : Set α) {s₁ s₁' s₂ s₂' : Set α} (h : s₁ ⊆ s₂) (h' : s₁' ⊆ s₂') :
-    t.ite s₁ s₁' ⊆ t.ite s₂ s₂' :=
-  fun _ h2 =>
-    match h2 with
-    | Or.inl h3 => Or.inl ⟨h h3.1, h3.2⟩
-    | Or.inr h3 => Or.inr ⟨h' h3.1, h3.2⟩
+theorem Set.ite_mono (t : Set α) {s₁ s₁' s₂ s₂' : Set α}
+  (h : s₁ ⊆ s₂) (h' : s₁' ⊆ s₂'):
+  t.ite s₁ s₁' ⊆ t.ite s₂ s₂' := λ _ h2 =>
+  match h2 with
+  | Or.inl ⟨hl, hr⟩ => Or.inl ⟨h hl, hr⟩
+  | Or.inr ⟨hl, hr⟩ => Or.inr ⟨h' hl, hr⟩
 
 /-
   ### Set theoretic (partial) functions
@@ -53,8 +60,8 @@ notation:20 α " →ˢ " β => Set (α × β)
 
 def id: α →ˢ α := {p | p.1 = p.2}
 
-theorem mem_id:
-  (a, b) ∈ id ↔ a = b := Iff.rfl
+theorem mem_id: (a, b) ∈ id ↔ a = b :=
+  Iff.rfl
 
 def comp (f g: α →ˢ α): α →ˢ α :=
   {x | ∃z, (x.1, z) ∈ f ∧ (z, x.2) ∈ g}
@@ -62,44 +69,31 @@ def comp (f g: α →ˢ α): α →ˢ α :=
 infixl:90 " ○ " => SFun.comp
 
 theorem mem_comp {f g: α →ˢ α}:
-  x ∈ f ○ g ↔ ∃z, (x.1, z) ∈ f ∧ (z, x.2) ∈ g := Iff.rfl
+  x ∈ f ○ g ↔ ∃z, (x.1, z) ∈ f ∧ (z, x.2) ∈ g :=
+  Iff.rfl
 
 theorem comp_mono {α: Type} {f g h k : Set (α × α)}
-  (h₁ : f ⊆ h) (h₂ : g ⊆ k): f ○ g ⊆ h ○ k :=
-  fun _ ⟨z, h, h'⟩ => ⟨z, h₁ h, h₂ h'⟩
+  (hfh : f ⊆ h) (hgk : g ⊆ k): f ○ g ⊆ h ○ k :=
+  λ _ ⟨z, h, h'⟩ => ⟨z, hfh h, hgk h'⟩
 
 theorem comp_id {f: α →ˢ α}: f ○ id = f := by
   funext x
   apply eq_iff_iff.mpr
-  apply Iff.intro
+  unfold comp
+  constructor
+  . intro ⟨z, h1, h2⟩
+    apply mem_id.mp h2 ▸ h1
   . intro h
-    unfold comp at h
-    match h with
-    | Exists.intro z h =>
-      match h with
-      | And.intro hl hr =>
-        rw [mem_id] at hr
-        rw [hr] at hl
-        exact hl
-  . intro h
-    unfold comp
-    exact Exists.intro x.2 (And.intro h rfl)
+    exact ⟨x.2, h, rfl⟩
 
 theorem id_comp {f: α →ˢ α}: id ○ f = f := by
   funext x
   apply eq_iff_iff.mpr
-  apply Iff.intro
+  unfold comp
+  constructor
+  . intro ⟨z, h1, h2⟩
+    apply mem_id.mp h1 ▸ h2
   . intro h
-    unfold comp at h
-    match h with
-    | Exists.intro z h =>
-      match h with
-      | And.intro hl hr =>
-        rw [mem_id] at hl
-        rw [hl.symm] at hr
-        exact hr
-  . intro h
-    unfold comp
-    exact Exists.intro x.1 (And.intro rfl h)
+    exact ⟨x.1, rfl, h⟩
 
 end SFun
