Semantics/KnasterTarski.lean
@@ -10,37 +10,37 @@ class PartialOrder (α: Type) extends LE α, LT α where
   le_iff_le_not_le: ∀ a b: α, a < b ↔ a ≤ b ∧ ¬b ≤ a
   le_antisymm: ∀ a b: α, a ≤ b → b ≤ a → a = b
 
-theorem PartialOrder.le_rfl [PartialOrder α] {a: α}: a ≤ a := le_refl a
+theorem PartialOrder.le_rfl [PartialOrder α] {a: α}:
+  a ≤ a :=
+  le_refl a
 
 theorem Set.le_def {α : Type} (A B : Set α) :
   A ≤ B ↔ A ⊆ B := Iff.rfl
 
 instance Set.LT (α: Type): LT (Set α) :=
   {
-    lt := fun A B => A ⊆ B ∧ A ≠ B
+    lt := λ a b => a ⊆ b ∧ a ≠ b
   }
 
-theorem Set.lt_def {α : Type} (A B : Set α) :
-  A < B ↔ A ⊆ B ∧ A ≠ B := Iff.rfl
+theorem Set.lt_def {α : Type} (a b : Set α):
+  a < b ↔ a ⊆ b ∧ a ≠ b :=
+  Iff.rfl
 
 instance Set.partialOrder: PartialOrder (Set α) :=
   {
-    le := fun A B => A ⊆ B,
-    lt := fun A B => A ⊆ B ∧ A ≠ B,
-    le_refl := fun _ _ ha => ha,
-    le_antisymm := fun _ _ h1 h2 => Subset.antisymm h1 h2,
+    le := λ a b => a ⊆ b,
+    lt := λ a b => a ⊆ b ∧ a ≠ b,
+    le_refl := λ _ _ ha => ha,
+    le_antisymm := λ _ _ h1 h2 => Subset.antisymm h1 h2,
     le_iff_le_not_le := by {
-      intro a b
-      apply Iff.intro
-      . intro h
-        exact ⟨h.1, fun h' => h.2 (Subset.antisymm h.1 h')⟩
-      . intro h
-        cases h with
-        | intro h1 h2 =>
-          rw [lt_def, le_def] at *
-          exact And.intro h1 (fun h3 => h2 $ Subset.from_eq h3.symm)
+      intro _ _
+      constructor
+      . intro ⟨h1, h2⟩
+        exact ⟨h1, λ h' => h2 $ Subset.antisymm h1 h'⟩
+      . intro ⟨h1, h2⟩
+        exact ⟨h1, λ h' => h2 $ Subset.from_eq h'.symm⟩
     }
-    le_trans := fun _ _ _ h1 h2 _ ha => h2 (h1 ha)
+    le_trans := λ _ _ _ h1 h2 _ ha => h2 (h1 ha)
   }
 
 class CompleteLattice (α: Type) extends PartialOrder α where
@@ -54,9 +54,9 @@ theorem inf_unique {α: Type} [CompleteLattice α] (s: Set α) (a b: α)
 
 instance Set.completeLattice: CompleteLattice (Set α) :=
   {
-    Inf := fun s => {x | ∀ A ∈ s, x ∈ A},
-    Inf_le := fun _ x hx _ ha => ha x hx,
-    le_Inf := fun _ _ h _ hb _ hd => h _ hd hb
+    Inf := λ s => {x | ∀ A ∈ s, x ∈ A},
+    Inf_le := λ _ x hx _ ha => ha x hx,
+    le_Inf := λ _ _ h _ hb _ hd => h _ hd hb
   }
 
 /-
@@ -89,20 +89,19 @@ def monotone {α β: Type} [PartialOrder α] [PartialOrder β]
   ∀a b, a ≤ b → f a ≤ f b
 
 theorem monotone_id {α: Type} [PartialOrder α]:
-  monotone (fun a: α => a) := fun _ _ h => h
+  monotone (λ a: α => a) := λ _ _ h => h
 
 theorem monotone_const {α β: Type} [PartialOrder α]
     [PartialOrder β] (b: β):
-  monotone (fun _: α => b) := fun _ _ _ => PartialOrder.le_refl b
+  monotone (λ _: α => b) := λ _ _ _ => PartialOrder.le_refl b
 
 theorem monotone_union {α β: Type} [PartialOrder α]
     (f g: α → Set β) (hf: monotone f) (hg: monotone g):
-  monotone (fun a => f a ∪ g a) :=
-  by
-    intro a₁ a₂ ha b hb
-    cases hb with
-    | inl h => exact Or.inl (hf a₁ a₂ ha h)
-    | inr h => exact Or.inr (hg a₁ a₂ ha h)
+  monotone (λ a => f a ∪ g a) := by
+  intro a a' ha b hb
+  match hb with
+  | Or.inl h => exact Or.inl (hf a a' ha h)
+  | Or.inr h => exact Or.inr (hg a a' ha h)
 
 /-
 ## The Knaster-Tarski Fixpoint Theorem
@@ -113,7 +112,7 @@ namespace Fix
 theorem lfp_eq {α: Type} [CompleteLattice α] (f: α → α)
     (hf: monotone f): lfp f = f (lfp f) :=
   let h: f (lfp f) ≤ lfp f :=
-    le_lfp (fun a h => PartialOrder.le_trans _ _ _ (hf _ a $ lfp_le h) h)
+    le_lfp (λ a h => PartialOrder.le_trans _ _ _ (hf _ a $ lfp_le h) h)
   PartialOrder.le_antisymm _ _ (lfp_le $ hf _ _ h) h
 
 end Fix
